Logic/AutoProver/ProofSearch.lean
@@ -50,13 +50,13 @@ open Qq Lean Elab Meta Tactic Litform Litform.Meta
 #check TwoSided.Derivation
 
 set_option linter.unusedVariables false in
-abbrev DerivationQ {F : Q(Type u)} (ls : Q(LogicSymbol $F)) (gz : Q(Gentzen.{u,v} $F)) (L R : List (Lit F)) :=
-  Q(TwoSided.Derivation $(Denotation.toExprₗ (denotation F ls) L) $(Denotation.toExprₗ (denotation F ls) R))
+abbrev DerivationQ {F : Q(Type u)} (instLS : Q(LogicSymbol $F)) (instGz : Q(Gentzen.{u,v} $F)) (L R : List (Lit F)) :=
+  Q(TwoSided.Derivation $(Denotation.toExprₗ (denotation F instLS) L) $(Denotation.toExprₗ (denotation F instLS) R))
 
 namespace DerivationQ
 open Denotation
 
-variable {F : Q(Type u)} {ls : Q(LogicSymbol $F)} {gz : Q(Gentzen.{u, v} $F)} (L R : List (Lit F))
+variable {F : Q(Type u)} {instLS : Q(LogicSymbol $F)} {instGz : Q(Gentzen.{u, v} $F)} (L R : List (Lit F))
 
 def DEq {F : Q(Type*)} : Lit F → Lit F → MetaM Bool
   | Litform.atom e,  Litform.atom e'  => Lean.Meta.isDefEq e e'
@@ -71,106 +71,106 @@ def DEq {F : Q(Type*)} : Lit F → Lit F → MetaM Bool
 def DMem {F : Q(Type*)} (p : Lit F) (Δ : List (Lit F)) : MetaM Bool :=
   Δ.foldrM (fun q ih => return (←DEq p q) || ih) false
 
-def rotateLeft {p : Lit F} (d : DerivationQ ls gz (L ++ [p]) R) : DerivationQ ls gz (p :: L) R :=
-  letI := denotation F ls
+def rotateLeft {p : Lit F} (d : DerivationQ instLS instGz (L ++ [p]) R) : DerivationQ instLS instGz (p :: L) R :=
+  letI := denotation F instLS
   let x : Q(TwoSided.Derivation
-    ($(Denotation.toExprₗ (denotation F ls) L) ++ [$(toExpr F p)])
-    $(Denotation.toExprₗ (denotation F ls) R)) := d
+    ($(Denotation.toExprₗ (denotation F instLS) L) ++ [$(toExpr F p)])
+    $(Denotation.toExprₗ (denotation F instLS) R)) := d
   q(Gentzen.rotateLeft $x)
 
-def rotateRight {p : Lit F} (d : DerivationQ ls gz L (R ++ [p])) : DerivationQ ls gz L (p :: R) :=
-  letI := denotation F ls
+def rotateRight {p : Lit F} (d : DerivationQ instLS instGz L (R ++ [p])) : DerivationQ instLS instGz L (p :: R) :=
+  letI := denotation F instLS
   let x : Q(TwoSided.Derivation
-    $(Denotation.toExprₗ (denotation F ls) L)
-    ($(Denotation.toExprₗ (denotation F ls) R) ++ [$(toExpr F p)])) := d
+    $(Denotation.toExprₗ (denotation F instLS) L)
+    ($(Denotation.toExprₗ (denotation F instLS) R) ++ [$(toExpr F p)])) := d
   q(Gentzen.rotateRight $x)
 
-def verum : DerivationQ ls gz L (⊤ :: R) := q(Gentzen.verum _ _)
+def verum : DerivationQ instLS instGz L (⊤ :: R) := q(Gentzen.verum _ _)
 
-def falsum : DerivationQ ls gz (⊥ :: L) R := q(Gentzen.falsum _ _)
+def falsum : DerivationQ instLS instGz (⊥ :: L) R := q(Gentzen.falsum _ _)
 
-def rEmLeftOfEq {p : Lit F} : MetaM (DerivationQ ls gz (p :: L) R) :=
-  letI := denotation F ls
-  do let some h ← Denotation.memList? (denotation F ls) p R | throwError m! "failed to derive {p} ∈ {R}"
+def rEmLeftOfEq {p : Lit F} : MetaM (DerivationQ instLS instGz (p :: L) R) :=
+  letI := denotation F instLS
+  do let some h ← Denotation.memList? (denotation F instLS) p R | throwError m! "failed to derive {p} ∈ {R}"
      return q(Gentzen.rEmLeft $h)
 
-def rEmRightOfEq {p : Lit F} : MetaM (DerivationQ ls gz L (p :: R)) :=
-  letI := denotation F ls
-  do let some h ← Denotation.memList? (denotation F ls) p L | throwError m! "failed to derive {p} ∈ {R}"
+def rEmRightOfEq {p : Lit F} : MetaM (DerivationQ instLS instGz L (p :: R)) :=
+  letI := denotation F instLS
+  do let some h ← Denotation.memList? (denotation F instLS) p L | throwError m! "failed to derive {p} ∈ {R}"
      return q(Gentzen.rEmRight $h)
 
-def rNegLeft {p : Lit F} (d : DerivationQ ls gz L (R ++ [p])) : DerivationQ ls gz (~p :: L) R :=
-  letI := denotation F ls
+def rNegLeft {p : Lit F} (d : DerivationQ instLS instGz L (R ++ [p])) : DerivationQ instLS instGz (~p :: L) R :=
+  letI := denotation F instLS
   let d : Q(TwoSided.Derivation
-    $(Denotation.toExprₗ (denotation F ls) L)
-    ($(Denotation.toExprₗ (denotation F ls) R) ++ [$(toExpr F p)])) := d
+    $(Denotation.toExprₗ (denotation F instLS) L)
+    ($(Denotation.toExprₗ (denotation F instLS) R) ++ [$(toExpr F p)])) := d
   q(Gentzen.rNegLeft $d)
 
-def rNegRight {p : Lit F} (d : DerivationQ ls gz (L ++ [p]) R) : DerivationQ ls gz L (~p :: R) :=
-  letI := denotation F ls
+def rNegRight {p : Lit F} (d : DerivationQ instLS instGz (L ++ [p]) R) : DerivationQ instLS instGz L (~p :: R) :=
+  letI := denotation F instLS
   let d : Q(TwoSided.Derivation
-    ($(Denotation.toExprₗ (denotation F ls) L) ++ [$(toExpr F p)])
-    $(Denotation.toExprₗ (denotation F ls) R)) := d
+    ($(Denotation.toExprₗ (denotation F instLS) L) ++ [$(toExpr F p)])
+    $(Denotation.toExprₗ (denotation F instLS) R)) := d
   q(Gentzen.rNegRight $d)
 
-def rAndLeft {p q : Lit F} (d : DerivationQ ls gz (L ++ [p, q]) R) : DerivationQ ls gz (p ⋏ q :: L) R :=
-  letI := denotation F ls
+def rAndLeft {p q : Lit F} (d : DerivationQ instLS instGz (L ++ [p, q]) R) : DerivationQ instLS instGz (p ⋏ q :: L) R :=
+  letI := denotation F instLS
   let d : Q(TwoSided.Derivation
-    ($(Denotation.toExprₗ (denotation F ls) L) ++ [$(toExpr F p), $(toExpr F q)])
-    $(Denotation.toExprₗ (denotation F ls) R)) := d
+    ($(Denotation.toExprₗ (denotation F instLS) L) ++ [$(toExpr F p), $(toExpr F q)])
+    $(Denotation.toExprₗ (denotation F instLS) R)) := d
   q(Gentzen.rAndLeft $d)
 
-def rAndRight {p q : Lit F} (dp : DerivationQ ls gz L (R ++ [p])) (dq : DerivationQ ls gz L (R ++ [q])) :
-    DerivationQ ls gz L (p ⋏ q :: R) :=
-  letI := denotation F ls
+def rAndRight {p q : Lit F} (dp : DerivationQ instLS instGz L (R ++ [p])) (dq : DerivationQ instLS instGz L (R ++ [q])) :
+    DerivationQ instLS instGz L (p ⋏ q :: R) :=
+  letI := denotation F instLS
   let dp : Q(TwoSided.Derivation
-    $(Denotation.toExprₗ (denotation F ls) L)
-    ($(Denotation.toExprₗ (denotation F ls) R) ++ [$(toExpr F p)])) := dp
+    $(Denotation.toExprₗ (denotation F instLS) L)
+    ($(Denotation.toExprₗ (denotation F instLS) R) ++ [$(toExpr F p)])) := dp
   let dq : Q(TwoSided.Derivation
-    $(Denotation.toExprₗ (denotation F ls) L)
-    ($(Denotation.toExprₗ (denotation F ls) R) ++ [$(toExpr F q)])) := dq
+    $(Denotation.toExprₗ (denotation F instLS) L)
+    ($(Denotation.toExprₗ (denotation F instLS) R) ++ [$(toExpr F q)])) := dq
   q(Gentzen.rAndRight $dp $dq)
 
-def rOrLeft {p q : Lit F} (dp : DerivationQ ls gz (L ++ [p]) R) (dq : DerivationQ ls gz (L ++ [q]) R) :
-    DerivationQ ls gz (p ⋎ q :: L) R :=
-  letI := denotation F ls
+def rOrLeft {p q : Lit F} (dp : DerivationQ instLS instGz (L ++ [p]) R) (dq : DerivationQ instLS instGz (L ++ [q]) R) :
+    DerivationQ instLS instGz (p ⋎ q :: L) R :=
+  letI := denotation F instLS
   let dp : Q(TwoSided.Derivation
-    ($(Denotation.toExprₗ (denotation F ls) L) ++ [$(toExpr F p)])
-    $(Denotation.toExprₗ (denotation F ls) R)) := dp
+    ($(Denotation.toExprₗ (denotation F instLS) L) ++ [$(toExpr F p)])
+    $(Denotation.toExprₗ (denotation F instLS) R)) := dp
   let dq : Q(TwoSided.Derivation
-    ($(Denotation.toExprₗ (denotation F ls) L) ++ [$(toExpr F q)])
-    $(Denotation.toExprₗ (denotation F ls) R)) := dq
+    ($(Denotation.toExprₗ (denotation F instLS) L) ++ [$(toExpr F q)])
+    $(Denotation.toExprₗ (denotation F instLS) R)) := dq
   q(Gentzen.rOrLeft $dp $dq)
 
-def rOrRight {p q : Lit F} (d : DerivationQ ls gz L (R ++ [p, q])) : DerivationQ ls gz L (p ⋎ q :: R) :=
-  letI := denotation F ls
+def rOrRight {p q : Lit F} (d : DerivationQ instLS instGz L (R ++ [p, q])) : DerivationQ instLS instGz L (p ⋎ q :: R) :=
+  letI := denotation F instLS
   let d : Q(TwoSided.Derivation
-    $(Denotation.toExprₗ (denotation F ls) L)
-    ($(Denotation.toExprₗ (denotation F ls) R) ++ [$(toExpr F p), $(toExpr F q)])) := d
+    $(Denotation.toExprₗ (denotation F instLS) L)
+    ($(Denotation.toExprₗ (denotation F instLS) R) ++ [$(toExpr F p), $(toExpr F q)])) := d
   q(Gentzen.rOrRight $d)
 
-def rImplyLeft {p q : Lit F} (dp : DerivationQ ls gz L (R ++ [p])) (dq : DerivationQ ls gz (L ++ [q]) R) :
-    DerivationQ ls gz ((p ⟶ q) :: L) R :=
-  letI := denotation F ls
+def rImplyLeft {p q : Lit F} (dp : DerivationQ instLS instGz L (R ++ [p])) (dq : DerivationQ instLS instGz (L ++ [q]) R) :
+    DerivationQ instLS instGz ((p ⟶ q) :: L) R :=
+  letI := denotation F instLS
   let dp : Q(TwoSided.Derivation
-    $(Denotation.toExprₗ (denotation F ls) L)
-    ($(Denotation.toExprₗ (denotation F ls) R) ++ [$(toExpr F p)])) := dp
+    $(Denotation.toExprₗ (denotation F instLS) L)
+    ($(Denotation.toExprₗ (denotation F instLS) R) ++ [$(toExpr F p)])) := dp
   let dq : Q(TwoSided.Derivation
-    ($(Denotation.toExprₗ (denotation F ls) L) ++ [$(toExpr F q)])
-    $(Denotation.toExprₗ (denotation F ls) R)) := dq
+    ($(Denotation.toExprₗ (denotation F instLS) L) ++ [$(toExpr F q)])
+    $(Denotation.toExprₗ (denotation F instLS) R)) := dq
   q(Gentzen.rImplyLeft $dp $dq)
 
-def rImplyRight {p q : Lit F} (d : DerivationQ ls gz (L ++ [p]) (R ++ [q])) : DerivationQ ls gz L ((p ⟶ q) :: R) :=
-  letI := denotation F ls
+def rImplyRight {p q : Lit F} (d : DerivationQ instLS instGz (L ++ [p]) (R ++ [q])) : DerivationQ instLS instGz L ((p ⟶ q) :: R) :=
+  letI := denotation F instLS
   let d : Q(TwoSided.Derivation
-    ($(Denotation.toExprₗ (denotation F ls) L) ++ [$(toExpr F p)])
-    ($(Denotation.toExprₗ (denotation F ls) R) ++ [$(toExpr F q)])) := d
+    ($(Denotation.toExprₗ (denotation F instLS) L) ++ [$(toExpr F p)])
+    ($(Denotation.toExprₗ (denotation F instLS) R) ++ [$(toExpr F q)])) := d
   q(Gentzen.rImplyRight $d)
 
-def deriveAux {F : Q(Type u)} (ls : Q(LogicSymbol $F)) (gz : Q(Gentzen.{u, v} $F)) :
-    ℕ → Bool → (L R : List (Lit F)) → MetaM (DerivationQ ls gz L R)
+def deriveAux {F : Q(Type u)} (instLS : Q(LogicSymbol $F)) (instGz : Q(Gentzen.{u, v} $F)) :
+    ℕ → Bool → (L R : List (Lit F)) → MetaM (DerivationQ instLS instGz L R)
   | 0,        _,     L,      R       => throwError m!"failed to prove {L} ⊢ {R}"
-  | s + 1,    true,  [],     R       => deriveAux ls gz s false [] R
+  | s + 1,    true,  [],     R       => deriveAux instLS instGz s false [] R
   | s + 1,    true,  p :: L, R       => do
     --logInfo m!"true: {s}"
     --logInfo (toString (p :: L) ++ " ⊢ " ++ toString R)
@@ -178,24 +178,24 @@ def deriveAux {F : Q(Type u)} (ls : Q(LogicSymbol $F)) (gz : Q(Gentzen.{u, v} $F
       rEmLeftOfEq L R
     else
     match p with
-    | ⊤ => return rotateLeft L R (← deriveAux ls gz s false (L ++ [⊤]) R)
+    | ⊤ => return rotateLeft L R (← deriveAux instLS instGz s false (L ++ [⊤]) R)
     | ⊥ => return falsum L R
-    | Litform.atom a => return rotateLeft L R (← deriveAux ls gz s false (L ++ [Litform.atom a]) R)
+    | Litform.atom a => return rotateLeft L R (← deriveAux instLS instGz s false (L ++ [Litform.atom a]) R)
     | ~p    => do
-      let d ← deriveAux ls gz s false L (R ++ [p])
+      let d ← deriveAux instLS instGz s false L (R ++ [p])
       return rNegLeft L R d
     | p ⋏ q => do
-      let d ← deriveAux ls gz s false (L ++ [p, q]) R
+      let d ← deriveAux instLS instGz s false (L ++ [p, q]) R
       return rAndLeft L R d
     | p ⋎ q => do
-      let dp ← deriveAux ls gz s false (L ++ [p]) R
-      let dq ← deriveAux ls gz s false (L ++ [q]) R
+      let dp ← deriveAux instLS instGz s false (L ++ [p]) R
+      let dq ← deriveAux instLS instGz s false (L ++ [q]) R
       return rOrLeft L R dp dq
     | p ⟶ q => do
-      let dp ← deriveAux ls gz s false L (R ++ [p])
-      let dq ← deriveAux ls gz s false (L ++ [q]) R
+      let dp ← deriveAux instLS instGz s false L (R ++ [p])
+      let dq ← deriveAux instLS instGz s false (L ++ [q]) R
       return rImplyLeft L R dp dq
-  | s + 1,    false, L,      []      => deriveAux ls gz s true L []
+  | s + 1,    false, L,      []      => deriveAux instLS instGz s true L []
   | s + 1,    false, L,      p :: R  => do
     --logInfo m!"false: {s}"
     --logInfo (toString L ++ " ⊢ " ++ toString [p :: R])
@@ -204,55 +204,97 @@ def deriveAux {F : Q(Type u)} (ls : Q(LogicSymbol $F)) (gz : Q(Gentzen.{u, v} $F
     else
     match p with
     | ⊤ => return verum L R
-    | ⊥ => return rotateRight L R (← deriveAux ls gz s true L (R ++ [⊥]))
-    | Litform.atom a => return rotateRight L R (← deriveAux ls gz s true L (R ++ [Litform.atom a]))
+    | ⊥ => return rotateRight L R (← deriveAux instLS instGz s true L (R ++ [⊥]))
+    | Litform.atom a => return rotateRight L R (← deriveAux instLS instGz s true L (R ++ [Litform.atom a]))
     | ~p    => do
-      let d ← deriveAux ls gz s true (L ++ [p]) R
+      let d ← deriveAux instLS instGz s true (L ++ [p]) R
       return rNegRight L R d
     | p ⋏ q => do
-      let dp ← deriveAux ls gz s true L (R ++ [p])
-      let dq ← deriveAux ls gz s true L (R ++ [q])
+      let dp ← deriveAux instLS instGz s true L (R ++ [p])
+      let dq ← deriveAux instLS instGz s true L (R ++ [q])
       return rAndRight L R dp dq
     | p ⋎ q => do
-      let d ← deriveAux ls gz s true L (R ++ [p, q])
+      let d ← deriveAux instLS instGz s true L (R ++ [p, q])
       return rOrRight L R d
     | p ⟶ q => do
-      let d ← deriveAux ls gz s true (L ++ [p]) (R ++ [q])
+      let d ← deriveAux instLS instGz s true (L ++ [p]) (R ++ [q])
       return rImplyRight L R d
 
-def derive {F : Q(Type u)} (ls : Q(LogicSymbol $F)) (gz : Q(Gentzen.{u, v} $F)) (s : ℕ) (L R : List (Lit F)) :
-    MetaM (DerivationQ ls gz L R) := deriveAux ls gz s true L R
+def derive {F : Q(Type u)} (instLS : Q(LogicSymbol $F)) (instGz : Q(Gentzen.{u, v} $F)) (s : ℕ) (L R : List (Lit F)) :
+    MetaM (DerivationQ instLS instGz L R) := deriveAux instLS instGz s true L R
 
 end DerivationQ
 
-def prove {F : Q(Type u)}
-    (ls : Q(LogicSymbol $F))
-    (sys : Q(System $F)) (_ : Q(LawfulGentzen.{u, v} $F))
-    (s : ℕ) (T : Q(Set $F)) (p : Q($F)) : MetaM Q($T ⊢ $p) :=
-  letI := Litform.Meta.denotation F ls; do
+def turnstile? (ty : Q(Prop)) : MetaM ((u : Level) × (F : Q(Type u)) × Q(Set $F) × Q($F)) := do
+  let ~q(@System.Provable $F $instLS $instSys $T $p) := ty | throwError "error: not a prop _ ⊢! _"
+  return ⟨_, F, T, p⟩
+
+
+
+
+
+
+section
+
+open Litform.Meta Denotation
+
+variable {F : Q(Type u)} (instLS : Q(LogicSymbol $F)) (instSys : Q(System $F)) (instLGz : Q(LawfulGentzen.{u, v} $F))
+
+
+def prove! (s : ℕ) (T : Q(Set $F)) (p : Q($F)) : MetaM Q($T ⊢! $p) :=
+  letI := Litform.Meta.denotation F instLS; do
   let lp : Litform.Meta.Lit F ← Denotation.denote F p
-  let d' : Q([] ⊢ᴳ [$p]) ← DerivationQ.derive ls q(LawfulGentzen.toGentzen) s [] [lp]
-  let b : Q($T ⊢ $p) := q(LawfulGentzen.toProof $d' $T)
+  let d' : Q([] ⊢ᴳ [$p]) ← DerivationQ.derive instLS q(LawfulGentzen.toGentzen) s [] [lp]
+  let b : Q($T ⊢! $p) := q(⟨LawfulGentzen.toProofOfNil $d' $T⟩)
   return b
 
-def prove! {F : Q(Type u)}
-    (ls : Q(LogicSymbol $F))
-    (sys : Q(System $F)) (_ : Q(LawfulGentzen.{u, v} $F))
-    (s : ℕ) (T : Q(Set $F)) (p : Q($F)) : MetaM Q($T ⊢! $p) :=
-  letI := Litform.Meta.denotation F ls; do
-  let lp : Litform.Meta.Lit F ← Denotation.denote F p
-  let d' : Q([] ⊢ᴳ [$p]) ← DerivationQ.derive ls q(LawfulGentzen.toGentzen) s [] [lp]
-  let b : Q($T ⊢! $p) := q(⟨LawfulGentzen.toProof $d' $T⟩)
+syntax termSeq := "[" (term,*) "]"
+
+def proofOfTurnstile? (T : Q(Set $F)) (e : Expr) : MetaM ((p : Q($F)) × Q($T ⊢ $p)) := do
+  let ⟨ty, h⟩ ← inferPropQ' e
+  let ⟨_, _, T', p⟩ ← turnstile? ty
+  if ← isDefEq T T' then return ⟨p, h⟩
+  else throwError m! "failed to find q such that {ty} == {T} ⊢ q"
+
+def proverL₀ (T : Q(Set $F)) (seq : Option (TSyntax `LO.AutoProver.termSeq)) :
+    letI := denotation F instLS
+    TermElabM ((L₀ : List (Lit F)) × Q(∀ q ∈ $(toExprₗ (denotation F instLS) L₀), $T ⊢! q)) :=
+  letI := denotation F instLS; do
+  let E ← (match seq with
+           | some seq =>
+             match seq with
+             | `(termSeq| [ $ss,* ] ) => do
+               ss.getElems.mapM (fun s => do
+                 proofOfTurnstile? instLS instSys T (← Term.elabTerm s none))
+             | _                      => return #[]
+           | _        => return #[])
+  let E : List ((p : Lit F) × Q($T ⊢ $(toExpr F p))) := Array.toList <| ← E.mapM fun e => do
+    let p : Lit F ← denote F e.1
+    return ⟨p, e.2⟩
+  let L₀ := E.map Sigma.fst
+  let H : Q(∀ q ∈ $(toExprₗ (denotation F instLS) L₀), $T ⊢! q)
+    ← listSigmaImpliment (denotation F instLS) (p := q(($T ⊢! ·))) E
+  return ⟨L₀, H⟩
+
+def proveL₀! (s : ℕ) (T : Q(Set $F)) (p : Q($F))
+    (L₀ : List (Lit F)) (H₀ : Q(∀ q ∈ $(toExprₗ (denotation F instLS) L₀), $T ⊢! q)) : MetaM Q($T ⊢! $p) :=
+  letI := denotation F instLS; do
+  let lp : Lit F ← Denotation.denote F p
+  let d' : Q($(toExprₗ (denotation F instLS) L₀) ⊢ᴳ [$p])
+    ← DerivationQ.derive instLS q(LawfulGentzen.toGentzen) s L₀ [lp]
+  let b : Q($T ⊢! $p) := q(LawfulGentzen.toProof₁! $d' $H₀)
   return b
 
-elab "tryProve" n:(num)? : tactic => do
+end
+
+elab "tautology" n:(num)? : tactic => do
   let s : ℕ :=
     match n with
     | some n => n.getNat
-    | none   => 16
+    | none   => 32
   let goalType ← Elab.Tactic.getMainTarget
-  let some ⟨.succ u, ty⟩ ← checkSortQ' goalType | throwError "error: not a type"
-  let ~q(@HasTurnstile.turnstile.{u} $F _ $ss $T $p) := ty | throwError "error: not a type 2"
+  let ty ← inferPropQ goalType
+  let ⟨u, F, T, p⟩ ← turnstile? ty
   let .some instLS ← trySynthInstanceQ (q(LogicSymbol.{u} $F) : Q(Type u))
     | throwError m! "error: failed to find instance LogicSymbol {F}"
   let .some instSys ← trySynthInstanceQ q(System $F)
@@ -260,50 +302,48 @@ elab "tryProve" n:(num)? : tactic => do
   let .some instLGZ ← trySynthInstanceQ q(LawfulGentzen.{u, u} $F)
     | throwError m! "error: failed to find instance LawfulGentzen {F}"
   --logInfo m! "start"
-  let b ← prove instLS instSys instLGZ s T p
-  Lean.Elab.Tactic.closeMainGoal b
-
-elab "try_prove" n:(num)? : tactic => do
-  let s : ℕ :=
-    match n with
-    | some n => n.getNat
-    | none   => 64
-  let goalType ← Elab.Tactic.getMainTarget
-  let ty ← inferPropQ goalType
-  let ~q(@System.Provable $F $j $jj $T $p) := ty | throwError "error: not a type 2"
-  let .some instLS ← trySynthInstanceQ (q(LogicSymbol.{u_1} $F) : Q(Type u_1))
-    | throwError m! "error: failed to find instance LogicSymbol {F}"
-  let .some instSys ← trySynthInstanceQ q(System $F)
-    | throwError m! "error: failed to find instance System {F}"
-  let .some instLGZ ← trySynthInstanceQ q(LawfulGentzen.{u_1, u_1} $F)
-    | throwError m! "error: failed to find instance LawfulGentzen {F}"
-  --logInfo m! "start"
   let b ← prove! instLS instSys instLGZ s T p
   Lean.Elab.Tactic.closeMainGoal b
 
+elab "prover" n:(num)? seq:(termSeq)? : tactic => do
+  let s : ℕ :=
+    match n with
+    | some n => n.getNat
+    | none   => 32
+  let goalType ← Elab.Tactic.getMainTarget
+  let ty ← inferPropQ goalType
+  let ⟨u, F, T, p⟩ ← turnstile? ty
+  let .some instLS ← trySynthInstanceQ (q(LogicSymbol.{u} $F) : Q(Type u))
+    | throwError m! "error: failed to find instance LogicSymbol {F}"
+  let .some instSys ← trySynthInstanceQ q(System $F)
+    | throwError m! "error: failed to find instance System {F}"
+  let .some instLGz ← trySynthInstanceQ q(LawfulGentzen.{u, u} $F)
+    | throwError m! "error: failed to find instance LawfulGentzen {F}"
+  let ⟨L₀, H₀⟩ ← proverL₀ instLS instSys T seq
+  let b ← proveL₀! instLS instSys instLGz s T p L₀ H₀
+  Lean.Elab.Tactic.closeMainGoal b
+
 section test
+
 open Propositional Formula
+
 variable (T : Theory ℕ)
 
-example : T ⊢! p ⋎ q ⋎ r ⋎ s ⟷ r ⋎ p ⋎ s ⋎ q ⋎ p := by try_prove
+example : T ⊢! p ⋎ q ⋎ r ⋎ s ⟷ r ⋎ p ⋎ s ⋎ q ⋎ p := by tautology
 
-example : T ⊢! p ⟷ p ⋎ p ⋎ p ⋎ p ⋎ p ⋎ p ⋎ p := by try_prove
+example : T ⊢! p ⟷ p ⋎ p ⋎ p ⋎ p ⋎ p ⋎ p ⋎ p := by tautology
 
-example : T ⊢! ((p ⟶ q) ⟶ p) ⟶ p := by try_prove
+example : T ⊢! ((p ⟶ q) ⟶ p) ⟶ p := by tautology
 
-example : T ⊢! (r ⟶ p) ⟶ ((p ⟶ q) ⟶ r) ⟶ p := by try_prove
+example : T ⊢! (r ⟶ p) ⟶ ((p ⟶ q) ⟶ r) ⟶ p := by tautology
 
-example : T ⊢! (p ⟶ q) ⋎ (q ⟶ p) := by try_prove
+example : T ⊢! (p ⟶ q) ⋎ (q ⟶ p) := by tautology
 
-/-
-example : T ⊢ p ⟶ p := by tryProve
+example : T ⊢! (p ⟷ q) ⟷ (~q ⟷ ~p) := by tautology
 
-example : T ⊢ p ⟶ p ⋎ q := by tryProve
+example (h : T ⊢! p ⟷ q) : T ⊢! ~q ⟷ ~p := by prover [h]
 
-example : T ⊢ q ⋎ p ⟷ p ⋎ q := by tryProve
-
-example : T ⊢ ((q ⟶ p) ⟶ q) ⟶ q := by tryProve
--/
+example (h : T ⊢! p ⟷ q) (hp : T ⊢! p) : T ⊢! q := by prover [h, hp]
 
 end test
 
